wip montanari

theories/unif.v
@@ -4,8 +4,14 @@ From elpi.apps Require Import derive derive.std.
 From HB Require Import structures.
 From det Require Import finmap ctx.
 From det Require Import lang.
+From det Require Import zify_ssreflect.
 
-Section s.
+From Stdlib Require Import FunInd.
+Require Import Recdef.
+Require Import Stdlib.Structures.OrdersEx.
+Require Import Stdlib.Wellfounded.Lexicographic_Product .
+
+
 (* Variable u: Unif. *)
 (* Notation matching := (matching u). *)
 (* Notation unify := (unify u). *)
@@ -13,6 +19,13 @@ Notation vars := vars_tm.
 
 Definition compare_var '(IV v1) '(IV v2) := 
   if v1 <= v2 then (IV v1, IV v2) else (IV v2, IV v1).
+
+Lemma compare_var_sym v1 v2: compare_var v1 v2 = compare_var v2 v1.
+Proof. 
+  case: v1 => v1; case: v2 => v2/=; rewrite leq_eqVlt.
+  rewrite eq_sym; case: eqP => //=[->|v21]//; first by rewrite if_same.
+  case: leqP => //=.
+Qed.
 
 Definition unify_var (s:Sigma) (v:V) arg := 
   if v \in vars_tm arg then None
@@ -24,53 +37,314 @@ Definition unify_var (s:Sigma) (v:V) arg :=
     end.
     (* Some s.[v <- arg]. *)
 
-Fixpoint unifier_help is_matchin n query pat s :=
-  let unifier_help := unifier_help is_matchin in
-  let query := deref s query in
-  let pat := deref s pat in
-  if query == pat then Some s
-  else
-  match n with
-  | 0 => None
-  | n.+1 =>
-    match pat with 
-    | Tm_V v' => unify_var s v' query
-    | Tm_D _ | Tm_P _ =>
-        match query with 
-        | Tm_V v => if is_matchin then None else unify_var s v pat
-        | _ => None
-        end
-    | Tm_App t1 t2 =>
-      match query with
-      | Tm_App tx ty => obind (unifier_help n ty t2) (unifier_help n tx t1 s)
-      | Tm_V v => if is_matchin then None else unify_var s v pat
-      | _ => None
-      end
-    end
-  end.
+Definition map_prod (T Q : Type) f (x: T * T) : (Q * Q) := (f x.1, f x.2).
+Definition map_prod1 (T Q R : Type) (g: R -> _ -> Q) f (x: T * T) := g (f x.1) (f x.2).
 
-Fixpoint size_tm t :=
+Definition seqT := seq (Tm * Tm).
+
+Definition sumL := foldr addn 0.
+
+Fixpoint count_vars (k:V) t :=
   match t with
-  | Tm_App f a => (size_tm f + size_tm a).+1
-  | _ => 1
+  | Tm_V v => v == k
+  | Tm_P _ | Tm_D _ => 0
+  | Tm_App f a => addn (count_vars k f) (count_vars k a)
   end.
 
-(* Definition vars_nb t1 t2 s := (size (vars_tmL t1) + size (vars_tmL t2) + #|` vars_sigma s|)%nat. *)
+Definition count_varsL k l := sumL (map (map_prod1 addn (count_vars k)) l).
 
-Definition unifier_help1 b t1 t2 s :=
-  omap (fun x => s + x) (unifier_help b (size_tm t1 + size_tm t2) t1 t2 s).
+Definition varsL l : fvS := varsU (map (map_prod1 fsetU vars_tm) l).
 
-Definition unifier_help2 b t1 t2 s := unifier_help1 b (deref s t1) (deref s t2) s.
+Definition nvar l := #|` [fset x in (varsL l) | count_varsL x l > 1]|.
 
-Definition matching := unifier_help2 true.
-Definition unify := unifier_help2 false.
+Lemma varsL_cons x xs: varsL (x :: xs) = map_prod1 fsetU vars_tm x `|` varsL xs.
+Proof. by []. Qed.
 
-Lemma compare_var_sym v1 v2: compare_var v1 v2 = compare_var v2 v1.
-Proof. 
-  case: v1 => v1; case: v2 => v2/=; rewrite leq_eqVlt.
-  rewrite eq_sym; case: eqP => //=[->|v21]//; first by rewrite if_same.
-  case: leqP => //=.
+Lemma map_prod1_comm T S (Q:choiceType) (R: _ -> _ -> S) (F: T -> Q) x y: 
+  commutative R -> map_prod1 R F (x,y) = map_prod1 R F (y,x).
+Proof. by move=> H; rewrite/map_prod1//. Qed.
+
+Lemma count_varsL_cons i x xs: 
+  count_varsL i (x :: xs) = (map_prod1 addn (count_vars i) x + count_varsL i xs)%N.
+Proof. by rewrite/count_varsL//. Qed.
+
+Lemma nvar_comm x1 x2 xs: nvar ((x1,x2) :: xs) = nvar ((x2, x1) :: xs).
+Proof.
+  rewrite /nvar; f_equal; apply/eqP/fset_eqP => i.
+  rewrite 2!inE/= 3![RHS]inE/=; f_equal.
+    by rewrite !varsL_cons map_prod1_comm//; apply/fsetUC.
+  rewrite !count_varsL_cons map_prod1_comm//; apply/addnC.
 Qed.
+
+Lemma nvar_sub h l : nvar l <= nvar (h :: l).
+Proof.
+  apply/fsubset_leq_card/fsubsetP.
+  move=> x; rewrite 2!inE/= 2!inE/= => /andP[H1 H2].
+  rewrite varsL_cons inE H1 orbT count_varsL_cons; lia.
+Qed.
+
+Lemma nvar_app f1 a1 f2 a2 tl: 
+  nvar ((Tm_App f1 a1, Tm_App f2 a2) :: tl) = nvar [:: (f1, f2), (a1, a2) & tl].
+Proof.
+  rewrite/nvar/count_varsL/=/map_prod1/=.
+  f_equal; apply/eqP/fset_eqP => x.
+  rewrite 2!inE/= 3![RHS]inE/=; f_equal.
+    rewrite !varsL_cons /map_prod1/= !inE; lia.
+  lia.
+Qed.
+
+Fixpoint app_nb t :=
+  match t with
+  | Tm_App f a => (app_nb f + app_nb a).+1
+  | Tm_V _ => 0
+  | Tm_D _ | Tm_P _ => 1
+  end.
+
+From Coq Require Import Wellfounded Inverse_Image.
+
+Definition nlhs (l:seqT) := sumL (map app_nb (map fst l)).
+
+Definition neqn (l:seqT) := size l.
+
+Definition measure l := (nvar l, nlhs l, neqn l).
+
+Definition lex_prod3 (T1 T2: Type) (F: T1 -> T1 -> Prop) (G : T2 -> T2 -> Prop) (x y: T1 * T2) := 
+  Relation_Operators.lexprod T1 (fun _ => T2) F (fun _ => G) (existT _ x.1 x.2) (existT _ y.1 y.2).
+
+Lemma wf_lex_prod3 T1 T2 F1 F2: well_founded F1 -> well_founded F2 -> 
+  well_founded (@lex_prod3 T1 T2 F1 F2).
+Proof. by move=> H1 H2; apply/wf_inverse_image/wf_lexprod. Qed.
+
+Lemma well_founded_lt: well_founded lt.
+Proof. apply/Nat_as_OT.lt_wf_0. Qed.
+
+Definition lex_prod2 := lex_prod3 lt lt.
+
+Lemma wf_lex_prod2: well_founded lex_prod2.
+Proof. apply/wf_lex_prod3/well_founded_lt/well_founded_lt. Qed.
+
+Definition lex_prod1:= lex_prod3 lex_prod2 lt.
+
+Lemma wf_lex_prod1: well_founded (lex_prod1).
+Proof. apply/wf_lex_prod3/well_founded_lt/wf_lex_prod2. Qed.
+
+Definition lex_seqT (t1 t2: seqT) := lex_prod1 (measure t1) (measure t2). 
+
+Lemma wf_lex_seqT : well_founded lex_seqT.
+Proof. apply/wf_inverse_image/wf_lex_prod1. Qed.
+
+Fixpoint derefkv k v (tm:Tm) :=
+  match tm with
+  | Tm_V k' => if k == k' then v else tm
+  | Tm_P _ | Tm_D _ => tm
+  | Tm_App h ag => Tm_App (derefkv k v h) (derefkv k v ag)
+  end.
+
+Lemma derefvk_in k v l t: k <> v ->
+  k \in vars (derefkv v l t) -> (k \in vars_tm l) || (k \in vars_tm t).
+Proof.
+  move=> H; elim: t => //=[v'|f Hf a Ha]; rewrite !inE.
+    by case: eqP => //=H1; subst; rewrite?inE => ->; rewrite//orbT.
+  by move=> /orP[/Hf|/Ha]/orP[]->//; rewrite !orbT.
+Qed.
+
+Lemma derefvk_in_varsL k v t2 tl:
+  k <> v ->
+  k \in [eta mem_seq (varsL [seq map_prod (derefkv v t2) i | i <- tl])] ->
+  (k \in vars t2) || (k \in varsL tl).
+Proof.
+  move=>H; elim: tl t2 => [|[t1 t2 tl IH]] l.
+    by rewrite inE.
+  rewrite /= !varsL_cons inE => /orP[|/IH]; last first.
+    by rewrite !inE => /orP[] ->//; rewrite !orbT.
+  by rewrite /map_prod1/= !inE => /orP[]/derefvk_in/orP[] => //->; rewrite//!orbT.
+Qed.
+
+(* Lemma count_vars_derefvk_sub :
+  count_vars k (derefkv v t t1) + count_vars k (derefkv v t t2) <=
+    count_vars k t + count_vars k t1.
+
+Lemma count_varsL_derefvk_sub v k t tl:
+  count_varsL k [seq map_prod (derefkv v t) i | i <- tl] <=
+    (v == k) + count_vars k t + count_varsL k tl.
+Proof.
+  elim: tl => -//=[t1 t2] L IH.
+  rewrite !count_varsL_cons /map_prod1/=.
+  rewrite 
+    rewrite /count_varsL//=.
+Admitted. *)
+
+Lemma deref_vk_not_in v t q: v \notin vars t -> v \notin vars (derefkv v t q).
+Proof.
+  move=> vt; elim: q => //=[v'|f Hf a Ha].
+    by case: eqP => //; rewrite inE; case: eqP.
+  by rewrite inE (negbTE Hf)//.
+Qed.
+
+Lemma deref_vkL_not_in v t tl: v \notin vars t ->
+  v \notin [eta mem_seq (varsL [seq map_prod (derefkv v t) i | i <- tl])].
+Proof.
+  move=> vt; elim: tl => //-[t1 t2 l IH]; rewrite /=varsL_cons !inE.
+  by rewrite (negbTE IH) orbF/= negb_or !deref_vk_not_in.
+Qed.
+
+(* Lemma count_varsL_derefvk_not_in:
+
+  count_varsL k [seq map_prod (derefkv v t) i | i <- tl] = count_varsL k tl. *)
+
+Lemma derefvk_sub v t tl:
+  v \notin vars_tm t ->
+  nvar [seq map_prod (derefkv v t) i | i <- tl] < nvar ((Tm_V v, t) :: tl).
+Proof.
+  (* rewrite /nvar => vt; apply/fproper_ltn_card; rewrite fproperE => //=.
+  apply/andP; split.
+    apply/fsubsetP => k; rewrite 2!inE/= 2!inE/=.
+    move=> /andP[H1 H2].
+    rewrite varsL_cons/= inE count_varsL_cons /map_prod1 /=!inE.
+    apply/andP; split.
+      by case: eqP => //= kv; apply/derefvk_in_varsL/H1.
+    case: eqP => ?; subst => /=.
+      by rewrite (negbTE (deref_vkL_not_in tl vt)) in H1.
+    
+    
+    
+
+    by apply/leq_trans/count_varsL_derefvk_sub.
+    have:= count_varsL_derefvk_sub v k t tl.
+    lia.
+    
+    case: eqP => //=.
+    rewrite /map_prod1.
+
+
+    f_equal.
+    rewrite 
+    Search (_ `<` _). *)
+
+Admitted.
+
+Lemma b1 t1 t2 tl:
+  (t1 == t2) = true -> lex_seqT tl ((t1, t2) :: tl).
+Proof.
+  move=> /eqP?; subst.
+  rewrite/lex_seqT.
+  rewrite/measure/=.
+  case: (boolP (nvar tl == nvar ((t2, t2) :: tl))) => [/eqP->| H].
+    case: (boolP (nlhs tl == nlhs ((t2, t2) :: tl))) => [/eqP->| H].
+      by constructor 2; auto => //=.
+    constructor 1 => /=; constructor 2 => /=.
+    move: H; rewrite /nlhs/=; lia.
+  (do 2 constructor 1) => /=.
+  move: H; set X:= nvar _; set Y:= nvar _.
+  have:= nvar_sub (t2,t2) tl; rewrite/Y/X.
+  move=> A B.
+  apply/leP; move: A B.
+  by rewrite leq_eqVlt; case: eqP.
+Qed.
+
+Lemma b2 tl p' v: lex_seqT ((Tm_V v, Tm_P p') :: tl) ((Tm_P p', Tm_V v) :: tl).
+Proof. rewrite/lex_seqT/measure/=nvar_comm; by constructor 1; constructor 2 => //=. Qed.
+
+Lemma b3 v d tl: lex_seqT ((Tm_V v, Tm_D d) :: tl) ((Tm_D d, Tm_V v) :: tl).
+Proof. rewrite/lex_seqT/measure/=nvar_comm; by constructor 1; constructor 2 => //=. Qed.
+
+Lemma b4 v t2 tl:
+  (v \in vars t2) = false ->
+  lex_seqT [seq map_prod (derefkv v t2) i | i <- tl]
+  ((Tm_V v, t2) :: tl).
+Proof.
+  rewrite/lex_seqT/measure/=.
+  do 2 constructor 1 => /=.
+  by apply/leP/derefvk_sub; rewrite H.
+Qed.
+
+Lemma b5 f1 f2 v tl: lex_seqT ((Tm_V v, Tm_App f1 f2) :: tl)
+  ((Tm_App f1 f2, Tm_V v) :: tl).
+Proof.
+  rewrite/lex_seqT/measure/=nvar_comm.
+  constructor 1; constructor 2 => /=.
+  rewrite/nlhs/=; lia.
+Qed.
+
+Lemma b6 f1 a1 f2 a2 tl:
+  lex_seqT [:: (f1, f2), (a1, a2) & tl]
+  ((Tm_App f1 a1, Tm_App f2 a2) :: tl).
+Proof.
+  rewrite/lex_seqT/measure/=.
+  constructor 1; rewrite nvar_app.
+  constructor 2; rewrite/=.
+  rewrite /nlhs/= !addnA//.
+Qed.
+
+Lemma measure_commV v1 v2 m:
+  measure ((Tm_V v1, Tm_V v2) :: m) = measure ((Tm_V v2, Tm_V v1) :: m).
+Proof. by rewrite/measure nvar_comm/=. Qed.
+
+Lemma lex_seqT_commV l v1 v2 m: 
+  lex_seqT l ((Tm_V v1, Tm_V v2) :: m) ->
+    lex_seqT l ((Tm_V v2, Tm_V v1) :: m).
+Proof. rewrite/lex_seqT measure_commV//. Qed.
+
+Opaque measure.
+
+Function montanari is_matching (l: seqT) {wf lex_seqT l} : option Sigma :=
+  match l with
+  | [::] => Some fmap0
+  | (t1, t2) :: tl => 
+    if t1 == t2 then montanari is_matching tl
+    else
+      match t1, t2 with
+      | Tm_App f1 a1, Tm_App f2 a2 => montanari is_matching ((f1, f2) :: (a1, a2) :: tl)
+      (* | Tm_V v, Tm_V v' =>
+        let: (v, v') := compare_var v v' in
+        let res := montanari is_matching (map (map_prod (derefkv v (Tm_V v'))) tl) in
+          omap (fun x => x.[v <- Tm_V v']) res *)
+      | Tm_V v, _ =>
+        if (v \in vars_tm t2)  then None
+        else 
+          let res := montanari is_matching (map (map_prod (derefkv v t2)) tl) in
+          omap (fun x => x.[v <- t2]) res
+      | _, Tm_V v => if is_matching then None else montanari is_matching ((t2, t1) :: tl)
+      | _, _ => None
+      end
+  end.
+Proof.
+  - move=> v l p tl t1 t2 ??; subst; apply: b1.
+  - move=> m l p tl t1 t2 p' ? v ??? /eqP// _ ?; subst; apply/b2.
+  - move=> m l p tl t1 t2 d ? v ??? /eqP// _ ?; subst; apply/b3.
+  (* - by move=> _ l p t t1 t2 v ? q ??? _ _; subst; apply/b4. *)
+  (* - by move=> _ l p t t1 t2 v ? q ??? _ _; subst; apply/b4. *)
+  (* - move=> _ l p tl t1 t2 v ? v' ???; case: eqP => // H _ v1 v2; subst.
+    rewrite/compare_var; case: v H => v; case: v' => v' H.
+    case: leq => -[??]; subst.
+      by apply/b4; rewrite !inE; case: eqP; congruence.
+    apply: lex_seqT_commV.
+    by apply/b4; rewrite !inE; case: eqP; congruence. *)
+  - move=> _ l p t t1 t2 v ????; subst; apply/b4.
+  - move=> m l p tl t1 t2 f1 f2 ? v ??? /eqP H ?; subst; apply/b5.
+  - move=> _ l p tl t1 t2 f1 a1 ? f2 a2 ??? /eqP H; subst; apply/b6.
+  - apply/wf_lex_seqT.
+Defined.
+
+Definition montanari_pair b t1 t2 := montanari b [::(t1,t2)].
+
+Goal montanari_pair false (Tm_D (ID 1)) (Tm_V (IV 1)) =
+   Some ctx.empty.[IV 1 <- Tm_D (ID 1)].
+Proof. by rewrite /montanari_pair !montanari_equation/=. Qed.
+
+Goal ~ montanari_pair true (Tm_D (ID 1)) (Tm_V (IV 1)).
+Proof. by rewrite /montanari_pair !montanari_equation/=. Qed.
+
+Goal forall b, montanari_pair b (Tm_V (IV 1)) (Tm_D (ID 1)).
+Proof. by move=> b; rewrite/montanari_pair !montanari_equation/=. Qed.
+
+Definition add_ (s:Sigma) r := omap (fun x => x + s) r.
+
+Definition montanari_deref b t1 t2 s := 
+  add_ s (montanari_pair b (deref s t1) (deref s t2)).
+
+Definition matching := montanari_deref true.
+Definition unify := montanari_deref false.
 
 Lemma omap_catf0 t: omap [eta catf empty] t = t.
 Proof. by case: t => //=?; rewrite cat0f. Qed.
@@ -79,47 +353,62 @@ Lemma omap_catf_refl (t:Sigma): omap [eta catf t] (Some t) = Some t.
 Proof. by rewrite/=; f_equal; apply/fmapP => k; rewrite fnd_cat if_same. Qed.
 
 Lemma unify_V_empty v t: v \notin vars_tm t -> 
-  unify (Tm_V v) t empty = unify_var empty v t.
+  unify (Tm_V v) t empty = Some empty.[v <- t].
 Proof.
-  rewrite/unify/unifier_help1/unifier_help2/unifier_help1 /= !deref_empty/= /unify_var omap_catf0.
-  case:t => //= v'. rewrite !inE eq_sym; case: eqP => //= ?.
-  case: eqP => //; first by congruence.
-  by rewrite compare_var_sym.
+  rewrite/unify/montanari_deref/montanari_pair montanari_equation/= !deref_empty.
+  case: eqP => [<-|vtd vt]; first by rewrite !inE eqxx.
+  by rewrite (negbTE vt) montanari_equation/= catf0.
+  (* rewrite /unify_var/compare_var. !montanari_equation/= (negbTE vt) /add_/= omap_catf0.
+  case: t vtd vt => //= x xs; rewrite inE => H; rewrite !push/=. *)
 Qed.
 
-Lemma unifier_help_refl h n t s: unifier_help h n t t s = Some s.
-Proof. by elim: n s t => [|n IH] s t//=; case D: deref; rewrite ?eqxx//?IH/=IH//. Qed.
+Lemma unifier_help_refl b t: montanari_pair b t t = Some fmap0.
+Proof. rewrite/montanari_pair montanari_equation eqxx montanari_equation//. Qed.
 
-Lemma unifier_help_refl1 b t s: unifier_help1 b t t s = Some s.
-Proof. by rewrite/unifier_help1 unifier_help_refl omap_catf_refl. Qed.
+Lemma unifier_help_refl1 b t s: montanari_deref b t t s = Some s.
+Proof. by rewrite /montanari_deref unifier_help_refl/= cat0f. Qed.
 
 Lemma unify_refl t s: unify t t s = Some s.
 Proof. apply/unifier_help_refl1. Qed.
 
-(* Lemma unify_help_ground_eq h n t1 t2 s s':
-  ground t1 -> ground t2 -> unifier_help h n t1 t2 s = Some s' -> t1 = t2.
-Proof.
-  elim: n t1 t2 s s' => //=[|n IH] t1 t2 s s' G1 G2; rewrite !ground_deref//.
-    by case: eqP => //.
-  case: t2 G2 => [p|d|v|f a]; case: t1 G1 => [p'|d'|v'|f' a']; rewrite ?ground_V//=; try by case: eqP.
-  rewrite !ground_app => /andP[Gf' Ga'] /andP[Gf Ga].
-  case: eqP => //= H.
-  case H1: unifier_help => [sx|]//=.
-  case H2: unifier_help => [sy|]//=.
-  by move=> [?]; subst; f_equal; apply/IH; eauto.
-Qed. *)
+Ltac montanari_ind b l :=
+  pattern b, l, (montanari b l);
+  eapply montanari_ind;
+  [
+    move=> {}b ?? | 
+    move=> {}b ? t1 t2 {}l ? EQ IH| 
+    move=> {}b ??? {}l ? []// EQ _ f1 a1 ? f2 a2 ? IH | 
+    move=> {}b ??? {}l ? []// EQ _ v ? t ? vt | 
+    move=> /={}b ??? {}l ? []// EQ _ v ? t ? []// vt _ IH| 
+    move=> {}b ??? {}l ? []// EQ _ t ? v ? NV M|
+    move=> {}b ??? {}l ? []// EQ _ t ? v ? NV []// ? _ IH | 
+    move=> {}b ??? {}l ? []// EQ _ t1 ? t2 ? H
+  ]; subst.
 
-Lemma unify_help_ground h n t1 t2 s: 
-  ground t1 -> ground t2 -> (t1 == t2) = (unifier_help h n t1 t2 s).
+Lemma montanari_cons_ground b t1 t2 l:
+  t1 != t2 -> ground t1 -> ground t2 -> ~~ montanari b ((t1, t2) :: l).
 Proof.
-  elim: n t1 t2 s => [|n IH] t1 t2 s/= G1 G2; rewrite !ground_deref//; case: eqP => //.
-  case: t2 G2 => [p|d|v|f a]; case: t1 G1 => [p'|d'|v'|f' a']//; rewrite?(ground_V,ground_app)//.
-  move=> /andP[gf' ga'] /andP[gf ga] H.
-  have:= IH _ _ s gf' gf; case: unifier_help => //s'; case: eqP => //=? _; subst.
-  have:= IH _ _ s' ga' ga; case: unifier_help => //s''; case: eqP => //; congruence.
+  elim: t1 t2 l => [p|d|v|f Hf a Ha] + l.
+    move=> [p'|d'|v'|f' a']//; rewrite montanari_equation//?ground_V// => /negbTE->//.
+    move=> [p'|d'|v'|f' a']//; rewrite montanari_equation//?ground_V// => /negbTE->//.
+    by move=> ?; rewrite ground_V.
+  move=> t2; rewrite montanari_equation => /[dup]+/negbTE->.
+  case: t2 => [p'|d'|v'|f' a']//; rewrite !(ground_app,ground_V)//.
+  move=> H /andP[gf ga] /andP[gf' ga'].
+  case: (boolP (f == f')) => [/eqP?|?]; last by apply: Hf.
+  subst; rewrite montanari_equation eqxx Ha//.
+  by apply/eqP => ?; subst; rewrite eqxx in H.
 Qed.
 
-Lemma unify_help_groundx b n t1 t2 s: 
+Lemma unify_help_ground b t1 t2: 
+  ground t1 -> ground t2 -> (t1 == t2) = (montanari_pair b t1 t2).
+Proof.
+  rewrite/montanari_pair.
+  case: eqP => //[->|]; first by rewrite 2!montanari_equation eqxx.
+  by move=> /eqP H1 G1 G2; apply/esym/negbTE/montanari_cons_ground.
+Qed.
+
+(* Lemma unify_help_groundx b n t1 t2 s: 
   ground t1 -> ground t2 -> t1 <> t2 -> unifier_help b n t1 t2 s = None.
 Proof.
   move=> G1 G2 H; have:= unify_help_ground b n s G1 G2.
@@ -138,11 +427,11 @@ Lemma unify_help2_groundx b t1 t2 s:
 Proof.
   move=> G1 G2 H; have:= unify_help1_groundx b s G1 G2 H.
   by rewrite/unifier_help2 !ground_deref//.
-Qed.
+Qed. *)
 
-Lemma unify_diff_ground t1 t2 s: 
+(* Lemma unify_diff_ground t1 t2 s: 
   ground t1 -> ground t2 -> t1 <> t2 -> unify t1 t2 s = None.
-Proof. by apply/unify_help2_groundx. Qed.
+Proof. by apply/unify_help2_groundx. Qed. *)
 
 Lemma isSomeP T x (P : option T) : P = Some x -> P.
 Proof. by move=> ->. Qed.
@@ -153,24 +442,26 @@ Proof. by move=> ->. Qed.
 Lemma isNoneP1 T (P : option T) : ~~ P -> P = None.
 Proof. case: P => //. Qed.
 
-
-Lemma match_help_unif n t1 t2 s s': 
-  unifier_help true n t1 t2 s = Some s' -> unifier_help false n t1 t2 s = Some s'.
+Lemma montanari_match_unif l s:
+  montanari true l = Some s -> montanari false l = Some s.
 Proof.
-  elim: n t1 t2 s s' => [|n IH]//= t1 t2 s s'.
-  case D1: deref => [p|d|v|f a];
-  case D2: deref => [p'|d'|v'|f' a']//=.
-  case: eqP => // _.
-  case u1: unifier_help => [sy|]//= u2.
-  rewrite (IH _ _ _ _ u1)//=.
-  by apply: IH.
+  move: false => b; move: s.
+  montanari_ind b l => s.
+  - by rewrite montanari_equation.
+  - by rewrite montanari_equation EQ; auto.
+  - by rewrite montanari_equation EQ; auto.
+  - by rewrite montanari_equation EQ vt.
+  - rewrite montanari_equation EQ vt; case M: montanari => [s'|]//=[?]; subst.
+    rewrite (IH s')//.
+  - by rewrite montanari_equation EQ; destruct t.
+  - by rewrite montanari_equation EQ; destruct t.
+  - by rewrite montanari_equation EQ; destruct t1, t2.
 Qed.
 
 Lemma match_unif t1 t2 s s': matching t1 t2 s = Some s' -> unify t1 t2 s = Some s'.
 Proof.
-  rewrite/matching/unify/unifier_help2/unifier_help1.
-  case U1: unifier_help => //=[sx][?]; subst.
-  by rewrite (match_help_unif U1)//.
+  rewrite/matching/unify/montanari_deref/montanari_pair; case M: montanari => //=[sx][?]; subst.
+  by rewrite (montanari_match_unif M).
 Qed.
 
 Lemma ground_vars_card t: ground t -> #|` vars_tm t | = 0.
@@ -179,68 +470,36 @@ Proof.
   by move=> /andP[/Hf/cardfs0_eq->]; rewrite fset0U.
 Qed.
 
-Lemma unify_fuel_ground n m b t1 t2 s:
-  ground t1 -> ground t2 ->
-  unifier_help b n t1 t2 s = unifier_help b m t1 t2 s.
-Proof.
-  move=> G1 G2; case: (boolP (t1 == t2)) => /eqP H; subst.
-    by rewrite !unifier_help_refl.
-  by rewrite !unify_help_groundx//.
-Qed.
-
-Lemma unif_fuel n m b t1 t2 s:
-  size_tm (deref s t1) + size_tm (deref s t2) <= n ->
-  size_tm (deref s t1) + size_tm (deref s t2) <= m ->
-  unifier_help b n t1 t2 s = unifier_help b m t1 t2 s.
-Proof.
-  elim: n m t1 t2 s => //=[|n IH] m t1 t2 s Hn Hm.
-    admit.
-  case: m Hm => [|m] Hm//=.
-    admit.
-  case: eqP => // D.
-  case D1: deref => [p|d|v|f a];
-  case D2: deref => [p'|d'|v'|f' a']//=.
-  case: (boolP (ground t1)) => G1.
-    move: D2; rewrite !ground_deref// => ?; subst.
-    move: G1; rewrite !ground_app => /andP[gf' ga'].
-    case: (boolP (ground t2)) => G2.
-      move: D1; rewrite !ground_deref// => ?; subst.
-      move: G2; rewrite !ground_app => /andP[gf ga].
-      rewrite (unify_fuel_ground _ m)//.
-      case: unifier_help => //=s'.
-      rewrite (unify_fuel_ground _ m)//.
-    move: Hn Hm => /=; rewrite deref_App/= addSn !ltnS => Hn Hm.
-    rewrite -(IH m)//=.
-      case U: unifier_help => [sx|]//=.
-      apply: IH.
-
-      admit.
-Admitted.
-
-Require Import Lia.
+Lemma add_eq0 a b: ((addn a b) == 0) = (a == 0) && (b == 0).
+Proof. case: a => //. Qed.
 
 (*SNIPT: unif_trans *)
 Lemma unif_trans t1 t2 t3 s: unify t1 t2 s -> unify t2 t3 s -> unify t1 t3 s.
 (*ENDSNIPT: unif_trans *)
 Proof.
-  (* pose N := (size (vars_tmL t1) + size (vars_tmL t2) + size (vars_tmL t3) + #|` vars_sigma s|)%nat.
-  rewrite/unify -(@unif_fuel N)%nat => //; last first.
-    by rewrite/N/vars_nb leq_add2r -addnA leq_add2l leq_addr.
-  move=> H1.
-  rewrite -(@unif_fuel N)%nat => //; last first.
-    by rewrite/N/vars_nb !leq_add2r leq_addl.
-  move=> H2.
-  rewrite -(@unif_fuel N)%nat => //; last first.
-    by rewrite/N/vars_nb !leq_add2r leq_addr.
-  move: H1 H2.
-  move: @N => /=.
-  remember (_ + _)%nat as n eqn:Hn; elim: n s t1 t2 t3 Hn => [|n IH] s t1 t2 t3 Hn.
-    admit. *)
 Admitted.
 
-Lemma unify_help_ext n t1 t2 s s':
+Lemma eq_app f1 a1 f2 a2:
+  (Tm_App f1 a1 == Tm_App f2 a2) = (f1 == f2) && (a1 == a2).
+Proof. do 3 case:eqP => //; congruence. Qed.
 
-  unifier_help false n t1 t2 s = Some s' ->
+Lemma montanariP b l s:
+  montanari b l = Some s -> all (map_prod1 (eq_op) (deref s)) l.
+Proof.
+  move: s; montanari_ind b l => s//=.
+  - by move/eqP: EQ => -> /IH; rewrite/map_prod1/=eqxx.
+  - by move=> /IH/=; rewrite {1 2 4}/map_prod1/= !deref_App eq_app => /and3P[->->].
+  - case M: montanari => [s'|]//=[?]; subst; move: M.
+    move=> /IH H.
+    apply/andP; split.
+      rewrite/map_prod1/=.
+      admit.
+    admit.
+  - move=> /IH/=/andP[+->]; rewrite andbT /map_prod1/= eq_sym//.
+Admitted.
+
+(* Lemma unify_help_ext n t1 t2 s s':
+  montanari_pair false n t1 t2 s = Some s' ->
     exists e : finMap lang_V__canonical__choice_Choice Tm,
       [disjoint domf e & domf s] /\ s' = s + e.
 Proof.
@@ -266,18 +525,69 @@ Proof.
     move=> [sy[D ?]][sz[R ?]]; subst.
     move: D; rewrite domf_cat fdisjointXU => /andP[S T].
     by exists (sz + sy); rewrite catfA domf_cat fdisjointUX R S.
-Admitted.
+Admitted. *)
 
 
-Lemma unif_ext t1 t2 s s': unify t1 t2 s = Some s' ->
+(* Lemma unif_ext t1 t2 s s': unify t1 t2 s = Some s' ->
   exists e, [disjoint domf e & domf s] /\ s' = s + e.
 Proof.
   rewrite/unify/unifier_help2/unifier_help1.
   case U: unifier_help => [sx|]//=[?]; subst.
   exists sx; split => //.
+Admitted. *)
+
+Inductive swap : seqT -> seqT -> Prop :=
+| swap0 : swap [::] [::]
+| swapC t1 t2 l1 l2: swap l1 l2 -> swap ((t1, t2) :: l1) ((t2,t1) :: l2)
+| swapS t1 t2 l1 l2: swap l1 l2 -> swap ((t1, t2) :: l1) ((t1,t2) :: l2).
+
+Lemma swap_map f l1 l2: swap l1 l2 -> swap (map (map_prod f) l1) (map (map_prod f) l2).
+Proof. by (elim => /=; clear) => [|t1 t2 l1 l2 H IH|t1 t2 l1 l2 H IH]; constructor. Qed.
+  
+
+Definition is_var t := match t with Tm_V _ => true | _ => false end.
+
+Lemma montanari_commS b l1 l2 s:
+  b = false -> swap l1 l2 -> montanari b l1 = Some s -> montanari b l2.
+Proof.
+  move: l2 s; montanari_ind b l1 => l2 s ?; subst => //.
+  - inversion 1; subst; rewrite montanari_equation//.
+  - inversion 1; subst; rewrite (montanari_equation _ (_ :: _))/= ?EQ; last by apply: IH.
+    by rewrite eq_sym EQ; apply: IH.
+  - inversion 1; subst; rewrite (montanari_equation _ ((Tm_App _ _, _) :: _)) ?EQ; last by apply: IH; do 2 constructor.
+    by rewrite eq_sym EQ; apply: IH; do 2 constructor.
+  - case M: montanari => //[s']+[?]; subst => S.
+    have {}IH := IH _ _ erefl (swap_map _ _) M.
+    inversion S; subst; rewrite montanari_equation?EQ?vt; last first;
+    have {IH} := IH _ H3; case IH: montanari => //[sz] _.
+    rewrite eq_sym EQ montanari_equation EQ vt IH/=.
+    destruct t; rewrite// inE; case: eqP => vv; subst.
+      by rewrite eqxx in EQ.
+    case N: montanari => //=.
+    admit.
+  - by move=> H; apply: IH => //; inversion H; subst; constructor.
 Admitted.
 
-Definition swaps_aux (s : Sigma) :=
+Lemma montanari_commN r b l1 l2:
+  r = None -> b = false -> swap l1 l2 -> montanari b l1 = r -> montanari b l2 = r.
+Proof.
+  pattern b, l1, (montanari b l1).
+  move: l2; montanari_ind b l1 => l2 s ?; subst => //.
+  - by move=> + M; inversion 1; subst; rewrite montanari_equation ?(eq_sym t2) EQ; eauto.
+  - by move=> + M; inversion 1; subst; rewrite montanari_equation ?(eq_sym (Tm_App f2 _)) EQ;
+    apply: IH => //; repeat constructor.
+  - inversion 1; subst; rewrite montanari_equation/= ?(eq_sym t) EQ ?vt//.
+    move=> _.
+  admit.
+  admit.
+  admit.
+  admit.
+  admit.
+  inversion 1; subst; rewrite montanari_equation ?(eq_sym t2) EQ; 
+  destruct t2, t1 => //.
+Admitted.
+
+(* Definition swaps_aux (s : Sigma) :=
   let d := filterf s (fun x => if s.[?x] is Some (Tm_V v) then true else false) in
   s.[\ domf d] + [fmap x : codom_vars d => Tm_V (get_father (val x) d)].
 
@@ -296,16 +606,16 @@ Proof. apply/fmapP => k; rewrite fnd_rem; case: (boolP (_ \in _)) => ks; rewrite
 Lemma swap_refl s: swap s s = s.
 Proof. by rewrite /swap restrictfT remf_all swaps_aux0 catf0. Qed.
 
-Definition is_var t := if t is (Tm_V _) then true else false.
+Definition is_var t := if t is (Tm_V _) then true else false. *)
 
 (* Definition principal_unifier sigma A : Prop :=
  unif sigma A /\ 
  forall tau, unif tau A -> forall s, tau (sigma s) = tau s. *)
 
-Axiom phi: Tm -> Tm -> Sigma.
+(* Axiom phi: Tm -> Tm -> Sigma.
 
 Axiom xx: forall t1 t2 s s', 
-  unify t1 t2 s = Some s' -> deref s' t1 = deref s' (deref (phi t1 t2) t1).
+  unify t1 t2 s = Some s' -> deref s' t1 = deref s' (deref (phi t1 t2) t1). *)
 
 (* f X X = f Z Y ====> {X = Z; Z = Y} *)
 (* f Z Y = f X X ====> {Y = X; Z = X} *)
@@ -348,6 +658,9 @@ Admitted. *)
 
 Lemma unif_sym t1 t2 s: unify t1 t2 s = unify t2 t1 s.
 Proof.
+  rewrite/unify/montanari_deref/montanari_pair.
+  case M: montanari => //=.
+  move=> /montanari_comm.
   rewrite/unify/unifier_help2/unifier_help1.
   move: (deref _ _) (deref _ _) => {}t1 {}t2.
   rewrite addnC; move: (_ + _)%nat => n.
